Rename 'free_variables' to 'closed'
Signed-off-by: Nicolas Iooss <nicolas.iooss_git@polytechnique.org>

closed_lterm.v
@@ -1,23 +1,23 @@
 Require Import Arith List lterm.
 
-(* Predicate: every free variable has an index below n *)
-Fixpoint fr_below (n: nat) (t: lterm) : Prop :=
+(** 1.2. Predicate: every free variable has an index below n *)
+Fixpoint closed_n (n: nat) (t: lterm) : Prop :=
   match t with
     | Var x => x < n
-    | Lambda u => fr_below (S n) u
-    | Apply u v => (fr_below n u) /\ (fr_below n v)
+    | Lambda u => closed_n (S n) u
+    | Apply u v => (closed_n n u) /\ (closed_n n v)
   end
 .
 
-(* Closed term *)
+(** Closed term *)
 Definition closed (t: lterm) : Prop :=
-  fr_below 0 t
+  closed_n 0 t
 .
 
-(* fr_below is still True when n increases *)
-Theorem fr_below_S:
+(** closed_n is still True when n increases *)
+Lemma closed_n_S:
   forall (t: lterm) (n: nat),
-  fr_below n t -> fr_below (S n) t.
+  closed_n n t -> closed_n (S n) t.
 Proof.
   induction t; simpl; intros i H.
     auto with arith.
@@ -27,9 +27,9 @@ Proof.
       apply IHt2; trivial.
 Save.
 
-Theorem fr_below_incr:
+Theorem closed_n_incr:
   forall (t: lterm) (n m: nat),
-  fr_below n t -> n <= m -> fr_below m t.
+  closed_n n t -> n <= m -> closed_n m t.
 Proof.
   intros t n; induction m; simpl; intros H H0.
     (* m = 0 *)
@@ -38,24 +38,24 @@ Proof.
     (* m = S m *)
     elim (le_lt_eq_dec n (S m)); trivial; clear H0; intro H0.
       (* n < S m *)
-      apply (fr_below_S t m).
+      apply (closed_n_S t m).
       apply IHm; trivial.
       auto with arith.
       (* n = S m *)
       rewrite <- H0; trivial.
 Save.
 
-(* forall u in ul, fr_below n u *)
-Fixpoint fr_below_list (n: nat) (ul: list lterm) : Prop :=
+(** forall u in ul, closed_n n u *)
+Fixpoint closed_n_list (n: nat) (ul: list lterm) : Prop :=
   match ul with
     | nil => True
-    | u :: l => (fr_below n u) /\ (fr_below_list n l)
+    | u :: l => (closed_n n u) /\ (closed_n_list n l)
   end
 .
 
-Lemma fr_below_list_forall:
+Theorem closed_n_list_forall:
   forall (n: nat) (ul: list lterm),
-  fr_below_list n ul -> (forall u: lterm, In u ul -> fr_below n u).
+  closed_n_list n ul -> (forall u: lterm, In u ul -> closed_n n u).
 Proof.
   intro n; induction ul; simpl; intros H u H0.
     contradict H0.
@@ -64,14 +64,14 @@ Proof.
       apply IHul; trivial.
 Save.
 
-(* fr_below_list is still True when n increases *)
-Theorem fr_below_list_S:
+(** closed_n_list is still True when n increases *)
+Theorem closed_n_list_S:
   forall (n: nat) (ul: list lterm),
-  fr_below_list n ul -> fr_below_list (S n) ul.
+  closed_n_list n ul -> closed_n_list (S n) ul.
 Proof.
   induction ul; simpl; trivial.
   intro H; destruct H.
   split.
-    apply fr_below_S; trivial.
+    apply closed_n_S; trivial.
     apply IHul; trivial.
 Save.
