Makefile
@@ -28,11 +28,11 @@ deps: $(SOURCES)
 	done | sort
 
 beta_reduction.vo: lterm.vo substitution.vo
-compiler_correct.vo: beta_reduction.vo compiler.vo free_variables.vo krivine.vo
+closed_lterm.vo: lterm.vo
+compiler_correct.vo: beta_reduction.vo compiler.vo closed_lterm.vo krivine.vo
 compiler_correct.vo: lterm.vo substitute_list.vo substitute_varlist.vo
-compiler.vo: free_variables.vo krivine.vo lterm.vo substitute_list.vo
-free_variables.vo: lterm.vo
-identity.vo: beta_reduction.vo compiler.vo compiler_correct.vo free_variables.vo krivine.vo lterm.vo
-substitute_list.vo: free_variables.vo lterm.vo substitution.vo substitute_varlist.vo
+compiler.vo: closed_lterm.vo krivine.vo lterm.vo substitute_list.vo
+identity.vo: beta_reduction.vo compiler.vo compiler_correct.vo closed_lterm.vo krivine.vo lterm.vo
+substitute_list.vo: closed_lterm.vo lterm.vo substitution.vo substitute_varlist.vo
 substitute_varlist.vo: lterm.vo substitution.vo
-substitution.vo: free_variables.vo lterm.vo
+substitution.vo: closed_lterm.vo lterm.vo
